src/Pipit.System.Base.fst
@@ -1,0 +1,76 @@
+(* Transition systems *)
+module Pipit.System.Base
+
+module C = Pipit.Context
+
+(* Step functions are relations so that we can express non-deterministic systems.
+   The recursive dependency for recursive binders XMu is easier to express as a
+   relation too. The result type is `prop`, rather than a computational boolean,
+   because composing the relations requires existential quantifiers. *)
+type stepfun (input: Type) (state: Type) (result: Type) =
+  (* Values of input variables *)
+  i: input ->
+  (* Starting state, or None for initial *)
+  s: option state ->
+  (* New state *)
+  s': state ->
+  (* Return value *)
+  r: result ->
+  prop
+
+let rec system_stepn
+  (#outer: nat)
+  (#input #state #result: Type)
+  (t: stepfun input state result)
+  (inputs: C.vector input (outer + 1))
+  (vs: C.vector result (outer + 1))
+  (s': state): prop =
+  match inputs, vs with
+  | [row], [r] -> t row None s' r
+  | (row :: inputs'), r :: vs' ->
+    exists (s'': state).
+      system_stepn #(outer - 1) t inputs' vs' s'' /\
+      t row (Some s'') s' r
+
+
+let system_map2 (#input #state1 #state2 #value1 #value2 #result: Type) (f: value1 -> value2 -> result)
+  (t1: stepfun input state1 value1)
+  (t2: stepfun input state2 value2):
+       stepfun input (state1 * state2) result =
+  (fun i s s' r ->
+     let s1, s2 = match s with
+         | None -> None, None
+         | Some (s1, s2) -> Some s1, Some s2
+     in
+     let s1', s2' = s' in
+     exists (r1: value1) (r2: value2).
+               t1 i s1 s1' r1 /\
+               t2 i s2 s2' r2 /\
+               r == f r1 r2)
+
+let system_pre (#input #state1 #v: Type) (init: v)
+  (t1: stepfun input state1 v):
+       stepfun input (state1 * v) v =
+  (fun i s s' r ->
+      let s1, v = match s with
+      | None -> None, init
+      | Some (s1, v) -> Some s1, v
+      in
+      let s1', v' = s' in
+      t1 i s1 s1' v' /\ r == v)
+
+let system_then (#input #state1 #state2 #v: Type)
+  (t1: stepfun input state1 v)
+  (t2: stepfun input state2 v):
+       stepfun input state2 v =
+  (fun i s s' r ->
+     match s with
+     | None -> exists s1' r'. t1 i None s1' r /\ t2 i None s' r'
+     | Some _ -> t2 i s s' r)
+
+let system_mu (#input #input' #state1 #v: Type)
+  (extend: input -> v -> input')
+  (t1: stepfun input' state1 v):
+       stepfun input state1 v =
+  (fun i s s' r ->
+      t1 (extend i r) s s' r)
