src/Pipit.System.Ind.fst
@@ -1,0 +1,3 @@
+module Pipit.System.Ind
+
+open Pipit.System.Base
